update interpreter2

theory/Interpreter1.thy
@@ -20,11 +20,11 @@ stack :: stack_state *)
 datatype bpf_state_ty = BPF_OK1 | BPF_Success1 | BPF_EFlag1 | BPF_Err1 | BPF_CU1
 
 datatype bpf_state1 =
-  BPF_st bpf_state_ty  u64 reg_map mem stack_state SBPFV u64 u64
+  BPF_st bpf_state_ty u64 u64 reg_map mem stack_state SBPFV u64 u64
                                                      
 fun bad_bpf_state1 :: "bpf_state_ty => bpf_state1" where
 "bad_bpf_state1 ty = (
-  BPF_st ty 0 (\<lambda> _. 0) (\<lambda> _. None) default_stack_state V1 0 0
+  BPF_st ty 0 0 (\<lambda> _. 0) (\<lambda> _. None) default_stack_state V1 0 0
 )"
 
 definition step1 :: "u64 \<Rightarrow> bpf_instruction \<Rightarrow> reg_map \<Rightarrow> mem \<Rightarrow> stack_state \<Rightarrow> SBPFV \<Rightarrow> u64 \<Rightarrow> u64 \<Rightarrow> bpf_state1" where
@@ -34,116 +34,116 @@ definition step1 :: "u64 \<Rightarrow> bpf_instruction \<Rightarrow> reg_map \<R
     case eval_alu32 bop d sop rs is_v1 of
     NOK \<Rightarrow> bad_bpf_state1 BPF_Err1 |
     OKN \<Rightarrow> bad_bpf_state1 BPF_EFlag1 |
-    OKS rs' \<Rightarrow> BPF_st BPF_OK1 (pc+1) rs' m ss sv (cur_cu+1) remain_cu ) |
+    OKS rs' \<Rightarrow> BPF_st BPF_OK1 (pc+1) (pc+1) rs' m ss sv (cur_cu+1) remain_cu ) |
 
   BPF_ALU64 bop d sop \<Rightarrow> (
     case eval_alu64 bop d sop rs is_v1 of
     NOK \<Rightarrow> bad_bpf_state1 BPF_Err1 |
     OKN \<Rightarrow> bad_bpf_state1 BPF_EFlag1 |
-    OKS rs' \<Rightarrow> BPF_st BPF_OK1 (pc+1) rs' m ss sv (cur_cu+1) remain_cu ) |
+    OKS rs' \<Rightarrow> BPF_st BPF_OK1 (pc+1) (pc+1) rs' m ss sv (cur_cu+1) remain_cu ) |
 
   BPF_ADD_STK i \<Rightarrow> (
     case eval_add64_imm_R10 i ss is_v1 of
     None \<Rightarrow> bad_bpf_state1 BPF_Err1 |
-    Some ss' \<Rightarrow> BPF_st BPF_OK1 (pc+1) rs m ss' sv (cur_cu+1) remain_cu ) |
+    Some ss' \<Rightarrow> BPF_st BPF_OK1 (pc+1) (pc+1) rs m ss' sv (cur_cu+1) remain_cu ) |
 
   BPF_LE dst imm \<Rightarrow> (
     case eval_le dst imm rs is_v1 of
     NOK \<Rightarrow> bad_bpf_state1 BPF_Err1 |
     OKN \<Rightarrow> bad_bpf_state1 BPF_EFlag1 |
-    OKS rs' \<Rightarrow> BPF_st BPF_OK1 (pc+1) rs' m ss sv (cur_cu+1) remain_cu ) |
+    OKS rs' \<Rightarrow> BPF_st BPF_OK1 (pc+1) (pc+1) rs' m ss sv (cur_cu+1) remain_cu ) |
 
   BPF_BE dst imm \<Rightarrow> (
     case eval_be dst imm rs is_v1 of
     NOK \<Rightarrow> bad_bpf_state1 BPF_Err1 |
     OKN \<Rightarrow> bad_bpf_state1 BPF_EFlag1 |
-    OKS rs' \<Rightarrow> BPF_st BPF_OK1 (pc+1) rs' m ss sv (cur_cu+1) remain_cu ) |
+    OKS rs' \<Rightarrow> BPF_st BPF_OK1 (pc+1) (pc+1) rs' m ss sv (cur_cu+1) remain_cu ) |
 
   BPF_NEG32_REG dst \<Rightarrow> (
     case eval_neg32 dst rs is_v1 of
     NOK \<Rightarrow> bad_bpf_state1 BPF_Err1 |
     OKN \<Rightarrow> bad_bpf_state1 BPF_EFlag1 |
-    OKS rs' \<Rightarrow> BPF_st BPF_OK1 (pc+1) rs' m ss sv (cur_cu+1) remain_cu ) |
+    OKS rs' \<Rightarrow> BPF_st BPF_OK1 (pc+1) (pc+1) rs' m ss sv (cur_cu+1) remain_cu ) |
 
   BPF_NEG64_REG dst \<Rightarrow> (
     case eval_neg64 dst rs is_v1 of
     NOK \<Rightarrow> bad_bpf_state1 BPF_Err1 |
     OKN \<Rightarrow> bad_bpf_state1 BPF_EFlag1 |
-    OKS rs' \<Rightarrow> BPF_st BPF_OK1 (pc+1) rs' m ss sv (cur_cu+1) remain_cu ) |
+    OKS rs' \<Rightarrow> BPF_st BPF_OK1 (pc+1) (pc+1) rs' m ss sv (cur_cu+1) remain_cu ) |
 
   BPF_LDX chk dst sop off \<Rightarrow> (
     case eval_load chk dst sop off rs m of
     None \<Rightarrow> bad_bpf_state1 BPF_EFlag1 |
-    Some rs' \<Rightarrow> BPF_st BPF_OK1 (pc+1) rs' m ss sv (cur_cu+1) remain_cu ) |
+    Some rs' \<Rightarrow> BPF_st BPF_OK1 (pc+1) (pc+1) rs' m ss sv (cur_cu+1) remain_cu ) |
 
   BPF_ST chk dst sop off \<Rightarrow> (
     case eval_store chk dst sop off rs m of
     None \<Rightarrow> bad_bpf_state1 BPF_EFlag1 |
-    Some m' \<Rightarrow> BPF_st BPF_OK1 (pc+1) rs m' ss sv (cur_cu+1) remain_cu ) |
+    Some m' \<Rightarrow> BPF_st BPF_OK1 (pc+1) (pc+1) rs m' ss sv (cur_cu+1) remain_cu ) |
 
   BPF_LD_IMM dst imm1 imm2  \<Rightarrow> (
     case eval_load_imm dst imm1 imm2 rs m of
     None \<Rightarrow> bad_bpf_state1 BPF_EFlag1 |
-    Some rs' \<Rightarrow> BPF_st BPF_OK1 (pc+1) rs' m ss sv (cur_cu+1) remain_cu ) |
+    Some rs' \<Rightarrow> BPF_st BPF_OK1 (pc+1) (pc+1) rs' m ss sv (cur_cu+1) remain_cu ) |
 
   BPF_PQR pop dst sop \<Rightarrow> (
     case eval_pqr32 pop dst sop rs is_v1 of
     NOK \<Rightarrow> bad_bpf_state1 BPF_Err1 |
     OKN \<Rightarrow> bad_bpf_state1 BPF_EFlag1 |
-    OKS rs' \<Rightarrow> BPF_st BPF_OK1 (pc+1) rs' m ss sv (cur_cu+1) remain_cu ) |
+    OKS rs' \<Rightarrow> BPF_st BPF_OK1 (pc+1) (pc+1) rs' m ss sv (cur_cu+1) remain_cu ) |
 
   BPF_PQR64 pop dst sop \<Rightarrow> (
     case eval_pqr64 pop dst sop rs is_v1 of
     NOK \<Rightarrow> bad_bpf_state1 BPF_Err1 |
     OKN \<Rightarrow> bad_bpf_state1 BPF_EFlag1 |
-    OKS rs' \<Rightarrow> BPF_st BPF_OK1 (pc+1) rs' m ss sv (cur_cu+1) remain_cu ) |
+    OKS rs' \<Rightarrow> BPF_st BPF_OK1 (pc+1) (pc+1) rs' m ss sv (cur_cu+1) remain_cu ) |
 
   BPF_PQR2 pop dst sop \<Rightarrow> (
     case eval_pqr64_2 pop dst sop rs is_v1 of
     NOK \<Rightarrow> bad_bpf_state1 BPF_Err1 |
     OKN \<Rightarrow> bad_bpf_state1 BPF_EFlag1 |
-    OKS rs' \<Rightarrow> BPF_st BPF_OK1 (pc+1) rs' m ss sv (cur_cu+1) remain_cu ) |
+    OKS rs' \<Rightarrow> BPF_st BPF_OK1 (pc+1) (pc+1) rs' m ss sv (cur_cu+1) remain_cu ) |
 
   BPF_HOR64_IMM dst imm \<Rightarrow> (
     case eval_hor64 dst imm rs is_v1 of
     NOK \<Rightarrow> bad_bpf_state1 BPF_Err1 |
     OKN \<Rightarrow> bad_bpf_state1 BPF_EFlag1 |
-    OKS rs' \<Rightarrow> BPF_st BPF_OK1 (pc+1) rs' m ss sv (cur_cu+1) remain_cu ) |
+    OKS rs' \<Rightarrow> BPF_st BPF_OK1 (pc+1) (pc+1) rs' m ss sv (cur_cu+1) remain_cu ) |
 
   BPF_JA off  \<Rightarrow>
-    BPF_st BPF_OK1 (pc + scast off + 1) rs m ss sv (cur_cu+1) remain_cu  |
+    BPF_st BPF_OK1 (pc+1) (pc + scast off + 1) rs m ss sv (cur_cu+1) remain_cu  |
 
   BPF_JUMP cond bpf_ireg snd_op off  \<Rightarrow> (
     if eval_jmp cond bpf_ireg snd_op rs  then
-      BPF_st BPF_OK1 (pc + scast off + 1) rs m ss sv (cur_cu+1) remain_cu 
+      BPF_st BPF_OK1 (pc+1) (pc + scast off + 1) rs m ss sv (cur_cu+1) remain_cu 
     else
-      BPF_st BPF_OK1 (pc + 1) rs m ss sv (cur_cu+1) remain_cu ) |
+      BPF_st BPF_OK1 (pc+1) (pc + 1) rs m ss sv (cur_cu+1) remain_cu ) |
 
   BPF_CALL_IMM src imm \<Rightarrow> (
     case eval_call_imm imm rs ss is_v1  of
     None \<Rightarrow> bad_bpf_state1 BPF_EFlag1 |
-    Some (pc, rs', ss') \<Rightarrow> BPF_st BPF_OK1 pc rs' m ss' sv (cur_cu+1) remain_cu ) |
+    Some (pc, rs', ss') \<Rightarrow> BPF_st BPF_OK1 (pc+1) pc rs' m ss' sv (cur_cu+1) remain_cu ) |
 
   BPF_CALL_REG src imm \<Rightarrow> (
     case eval_call_reg src imm rs ss is_v1 pc of
     None \<Rightarrow> bad_bpf_state1 BPF_EFlag1 |
-    Some (pc', rs', ss') \<Rightarrow> BPF_st BPF_OK1 pc' rs' m ss' sv (cur_cu+1) remain_cu ) |
+    Some (pc', rs', ss') \<Rightarrow> BPF_st BPF_OK1 (pc+1) pc' rs' m ss' sv (cur_cu+1) remain_cu ) |
   BPF_EXIT \<Rightarrow> (
     if call_depth ss = 0 then
       if cur_cu >  remain_cu then
         bad_bpf_state1 BPF_EFlag1
       else
-        BPF_st BPF_Success1 pc rs m ss sv cur_cu remain_cu
+        BPF_st BPF_Success1 0 pc rs m ss sv cur_cu remain_cu
     else (
       let (pc', rs', ss') = eval_exit rs ss is_v1 in
-        BPF_st BPF_OK1 pc' rs' m ss' sv (cur_cu+1) remain_cu ))
+        BPF_st BPF_OK1 (pc+1) pc' rs' m ss' sv (cur_cu+1) remain_cu ))
 )"
 
 fun bpf_interp1 :: "nat \<Rightarrow> bpf_bin \<Rightarrow> bpf_state1 \<Rightarrow> bpf_state1" where
 "bpf_interp1 0 _ _ = bad_bpf_state1 BPF_EFlag1 " | 
 "bpf_interp1 (Suc n) prog st  = (
   case st of
-  BPF_st ty pc rs m ss sv cur_cu remain_cu \<Rightarrow> (
+  BPF_st ty lpc pc rs m ss sv cur_cu remain_cu \<Rightarrow> (
     case ty of
     BPF_OK1 \<Rightarrow> (
     if INSN_SIZE*unat pc < length prog then
@@ -160,7 +160,7 @@ fun bpf_interp1 :: "nat \<Rightarrow> bpf_bin \<Rightarrow> bpf_state1 \<Rightar
 definition refine_bpf_state1 :: "bpf_state1 \<Rightarrow> bpf_state" where
 "refine_bpf_state1 st = (
   case st of
-  BPF_st ty pc rs m ss sv cur_cu remain_cu \<Rightarrow> (
+  BPF_st ty lpc pc rs m ss sv cur_cu remain_cu \<Rightarrow> (
     case ty of
     BPF_OK1 \<Rightarrow> BPF_OK pc rs m ss sv cur_cu remain_cu |
     BPF_Err1 \<Rightarrow> BPF_Err |
@@ -243,21 +243,21 @@ theorem bpf_interp1_equiv:
   subgoal for k l st0 st1 st
     apply simp
     apply (cases st0)
-    subgoal for x1 x2 x3 x4 x5 x6 x7 x8
+    subgoal for x1 x2 x3 x4 x5 x6 x7 x8 x9
       apply (simp add: refine_bpf_state1_def)
       apply (cases x1; simp)
-      apply (cases "INSN_SIZE * unat x2 < length l"; simp)
-      apply (cases "x8 \<le> x7"; simp)
-      apply (cases "bpf_find_instr (unat x2) l"; simp)
+      apply (cases "INSN_SIZE * unat x3 < length l"; simp)
+      apply (cases "x9 \<le> x8"; simp)
+      apply (cases "bpf_find_instr (unat x3) l"; simp)
       subgoal for a
-        apply (subgoal_tac "step x2 a x3 x4 x5 x6 x7 x8 = (refine_bpf_state1 (step1 x2 a x3 x4 x5 x6 x7 x8))")
+        apply (subgoal_tac "step x3 a x4 x5 x6 x7 x8 x9 = (refine_bpf_state1 (step1 x3 a x4 x5 x6 x7 x8 x9))")
          prefer 2
         subgoal
           using bpf_step1_equiv
           apply simp
           done
         apply simp
-        apply (cases "step1 x2 a x3 x4 x5 x6 x7 x8"; simp add: refine_bpf_state1_def)
+        apply (cases "step1 x3 a x4 x5 x6 x7 x8 x9"; simp add: refine_bpf_state1_def)
         done
       done
     done
